newio/DM.IIO.Refine.fst
@@ -1,0 +1,221 @@
+module DM.IIO.Refine
+
+open FStar.Classical.Sugar
+open FStar.List.Tot.Base
+open FStar.Tactics
+
+open Free
+open Free.IO
+open DM.IIO
+open Hist
+
+(** the post-condition is written over an output value and local trace, therefore,
+  `return_of` is not enough and we need predicates and lemmas that show that for 
+  each x that is a returned value by m, also exists a local trace **)
+  
+let rec trace_of (lt:trace) (m:iio 'a) (x:'a) =
+  match lt, m with
+  | _, Call GetTrace arg k -> exists h. trace_of lt (k h) x
+  | [], Return x' -> x == x'
+  | e::es, Call cmd arg k -> 
+     (let (| cmd', arg', res' |) = destruct_event e in 
+          (cmd' == cmd /\ arg == arg' /\ (trace_of es (k res') x)))
+  | _, _ -> False
+
+let exists_trace_of (x:'a) (m:iio 'a) =
+  exists lt. trace_of lt m x
+
+let rec lemma_return_of_implies_exists_trace_of (m:iio 'a) (x:'a) : 
+  Lemma
+    (requires (x `return_of` m))
+    (ensures (exists_trace_of x m)) =
+  match m with
+  | Return _ -> assert (trace_of [] m x)
+  | Call cmd arg k -> begin
+    eliminate exists r. (x `return_of` (k r)) returns (exists_trace_of x m) with _. begin
+      lemma_return_of_implies_exists_trace_of (k r) x;
+      assert (exists klt. trace_of klt (k r) x) by (assumption ());
+      eliminate exists klt. trace_of klt (k r) x returns (exists_trace_of x m) with _. begin
+        match cmd with
+        | GetTrace ->
+          introduce exists lt. (trace_of lt m x) with klt and begin
+            assert (exists (h: trace).
+              iio_wps GetTrace arg (fun lt r -> lt == [] /\ r == h) h /\ trace_of klt (k h) x)
+          end
+        | _ -> begin
+          let e = convert_call_to_event cmd arg r in
+          introduce exists lt. (trace_of lt m x) with (e::klt) and begin
+            assert (trace_of (e::klt) m x)
+          end
+        end
+      end
+    end
+  end
+
+unfold let cast_trace (h:trace) : iio_sig.res GetTrace = h
+
+#push-options "--z3rlimit 10"
+let rec lemma_theta_result_implies_post (m:iio 'a) (p:hist_post #event 'a) (h:trace) : 
+  Lemma 
+    (requires theta m p h) 
+    (ensures (forall x lt. trace_of lt m x ==> p lt x)) =
+    match m with
+    | Call GetTrace arg k -> begin
+      assert (theta (k h) p h);
+      lemma_theta_result_implies_post (k h) p h;
+      assert (forall x lt. trace_of lt (k h) x ==> p lt x);
+
+      introduce forall x lt. trace_of lt (Call GetTrace arg k) x ==> trace_of lt (k h) x with begin
+        introduce trace_of lt (Call GetTrace arg k) x ==> trace_of lt (k h) x with _. begin
+          
+          assert (iio_wps GetTrace arg (fun lt r -> lt == [] /\ r == h) h);
+          assert (trace_of lt (Call GetTrace arg k) x);
+          assert (trace_of lt (k h) x) by (
+            let h = nth_binder 3 in
+            let x = nth_binder (-7) in
+ //           let y = nth_binder (-15) in
+            binder_retype x;
+              norm [delta_only [`%trace_of];zeta];
+//              witness (`(`#h));
+            trefl ();
+//            let _ = ExtraTactics.apply_in x y in
+            dump "H");
+          admit ()
+        end
+      end;
+      assert (forall x lt. trace_of lt m x ==> p lt x)
+    end
+    | _ -> admit ()
+(**
+    | Return _ -> ()
+    | Call cmd arg k -> begin
+      introduce forall x lt. trace_of lt m x ==> p lt x with begin
+        introduce trace_of lt m x ==> p lt x with _. begin
+          let e::klt = lt in
+          let (| cmd', arg', res' |) = destruct_event e in
+          let p' = (hist_post_shift p [convert_call_to_event cmd arg res']) in
+          let h' = (convert_call_to_event cmd arg res' :: h) in
+          assert (theta (k res') p' h');
+          lemma_theta_result_implies_post (k res') p' h';
+          assert (trace_of klt (k res') x);
+          assert (p' klt x);
+          assert (p lt x)
+       end
+     end
+    end**)
+
+let respects (x:'a) (wp:hist #event 'a) : Type0 =
+  forall (h:trace) (p:hist_post #event 'a). wp p h ==> (exists (lt:trace). p lt x)
+
+let resp (wp:hist 'a) = x:'a{x `respects` wp}
+let resph (wp:hist 'a) = hist #event (resp wp) 
+
+(** and we show that return_of implies respects **)
+let lemma_return_of_implies_respects (d:dm 'a 'wp) :
+  Lemma (forall x. x `return_of` d ==> x `respects` 'wp) = 
+  assert ('wp `hist_ord` theta d);
+  introduce forall x. x `return_of` d ==> x `respects` 'wp with begin
+    introduce x `return_of` d ==> x `respects` 'wp with _. begin
+      lemma_return_of_implies_exists_trace_of d x;
+      Classical.forall_intro_2 (Classical.move_requires_2 (lemma_theta_result_implies_post d));
+      assert (x `respects` 'wp)
+    end
+  end
+
+unfold
+let refine_io (wp:hist 'a) (d:dm 'a wp) : iio (resp wp) =
+  lemma_return_of_implies_respects d;
+  free_subcomp _ (fun _ -> True) (fun x -> respects x wp) d
+
+unfold
+let cast_post0 (q:pure_post 'a) (p:hist_post (v:'a{q v})) : hist_post 'a =
+  (fun lt (r:'a) -> q r ==> p lt r)
+
+unfold
+let cast_post (wp:hist 'a) (p : hist_post (resp wp)) : hist_post 'a = 
+  cast_post0 (fun x -> x `respects` wp) p
+
+let refine_hist (wp:hist 'a) : resph wp = 
+  let newhist : hist0 (resp wp) = (fun p -> wp (cast_post wp p)) in
+  assert (hist_wp_monotonic newhist);
+  newhist
+
+let lemma_refine_hist_implies_weaken_post (wp:hist 'a) : Lemma (
+  forall (p:hist_post 'a) h. refine_hist wp p h ==> wp (cast_post wp p) h) = ()
+
+let lemma_cast_post0 (q:pure_post 'a) (p:hist_post (v:'a{q v})) :
+  Lemma (
+    let p2 : hist_post (v:'a{q v}) = fun lt r -> cast_post0 q p lt r in
+    p2 `hist_post_ord` p
+  ) = ()
+
+let rec lemma_io_subcomp
+  (q1:pure_post 'a) (q2:pure_post 'a)
+  (m : iio (v:'a{q1 v})) :
+  Lemma
+    (requires (forall x. q1 x /\ x `return_of` m ==> q2 x))
+    (ensures (theta m `hist_ord #_ #'a` theta (free_subcomp _ q1 q2 m))) =
+  match m with
+  | Return x -> assert (theta m `hist_ord #_ #'a` theta (free_subcomp _ q1 q2 m)) by (compute ())
+  | Call cmd arg k -> begin
+    let fst : iio_sig.res cmd -> hist (v:'a{q1 v}) = fun r -> theta (k r) in
+    let snd : iio_sig.res cmd -> hist (v:'a{q2 v}) = fun r -> theta (free_subcomp _ q1 q2 (k r)) in
+    calc (==) {
+      theta m;
+      == {}
+      theta (Call cmd arg k);
+      == { _ by (compute ()) } // unfold theta
+      hist_bind (iio_wps cmd arg) (fun r -> theta (k r));
+      == {}
+      hist_bind (iio_wps cmd arg) fst;
+    };
+    (** fst ==> snd /\ hist is monotonic **)
+    introduce forall (p:hist_post 'a) h. hist_bind (iio_wps cmd arg) fst p h ==> hist_bind (iio_wps cmd arg) snd p h with begin 
+      introduce forall (r:iio_sig.res cmd). (fst r `hist_ord #event #'a` snd r) with begin
+        lemma_io_subcomp q1 q2 (k r)
+      end
+    end;
+    calc (==) {
+      hist_bind (iio_wps cmd arg) snd;
+      == {}
+      hist_bind (iio_wps cmd arg) (fun r -> theta (free_subcomp _ q1 q2 (k r)));
+      == { _ by (compute ()) }
+      theta (Call cmd arg (fun r -> free_subcomp _ q1 q2 (k r)));
+      == { _ by (compute ()) }
+      theta (free_subcomp _ q1 q2 (Call cmd arg k));
+      == {}
+      theta (free_subcomp _ q1 q2 m);
+    }
+  end
+  
+
+let lemma_io_subcomp_2 (q:pure_post 'a) (m : iio 'a) :
+  Lemma 
+    (requires (forall x. x `return_of` m ==> q x))
+    (ensures (forall p h. theta m (cast_post0 q p) h ==> theta (free_subcomp _ (fun _ -> True) q m) p h)) =
+  introduce forall p h. (theta m (cast_post0 q p) h ==> theta (free_subcomp _ (fun _ -> True) q m) p h) with begin 
+    introduce theta m (cast_post0 q p) h ==> (theta (free_subcomp _ (fun _ -> True) q m) p h) with _. begin 
+      assert (theta m (cast_post0 q p) h);
+      lemma_io_subcomp (fun _ -> True) q m;
+      assert (theta (free_subcomp _ (fun _ -> True) q m) p h)
+    end
+  end
+
+let lemma_theta_cast_post_implies_theta_refine_io (d:dm 'a 'wp) :
+  Lemma (forall p h. theta d (cast_post 'wp p) h ==> theta (refine_io 'wp d) p h) =
+  lemma_return_of_implies_respects d;
+  lemma_io_subcomp_2 (fun x -> x `respects` 'wp) d
+  
+let lemma_refine_io_refine_hist (d:dm 'a 'wp) : 
+  Lemma (refine_hist 'wp `hist_ord` theta (refine_io 'wp d)) =
+  assert ('wp `hist_ord` theta d);
+  lemma_refine_hist_implies_weaken_post 'wp;
+  assert (forall p h. refine_hist 'wp p h ==> theta d (cast_post 'wp p) h);
+  lemma_theta_cast_post_implies_theta_refine_io d;
+  assert (forall p h. theta d (cast_post 'wp p) h ==> theta (refine_io 'wp d) p h)
+  
+let refine_dm (d:dm 'a 'wp) : dm (resp 'wp) (refine_hist 'wp) =
+  lemma_refine_io_refine_hist d;
+  refine_io 'wp d
+
+
